src/data-types/binary-tree/BST.dfy
@@ -1,0 +1,135 @@
+include "../list/List.dfy"
+
+// -------------------------- Datatype -------------------------- //
+
+datatype Leaf = Nil
+datatype BST<T> = Leaf | Node(left:BST<T>, data:T, right:BST<T>)
+
+// ---------------------- Function Methods ---------------------- //
+
+function method BST_Init() : (tree:BST<T>)
+  ensures bst_is_ordered(tree)
+{
+  Leaf
+}
+
+function method BST_Size(tree:BST<T>) : (n:int)
+  decreases tree
+{
+    match tree {
+      case Leaf => 0
+      case Node(left, x, right) => BST_Size(left) + 1 + BST_Size(right)
+    }
+}
+
+function method BST_Insert(tree:BST<T>, d:T) : (result:BST<T>)
+  decreases tree
+  requires bst_is_ordered(tree)
+  // Ensures que Result esté ordenado
+{
+  match tree {
+    case Leaf => Node(Leaf, d, Leaf)
+    case Node(left, x, right) => 
+      if (d < x) 
+        then Node(BST_Insert(left, d), x, right)
+      else Node(left, x, BST_Insert(right, d))
+  }
+}
+
+function method BST_InOrder(tree:BST<T>) : (result:List<T>)
+  decreases tree
+  requires bst_is_ordered(tree)
+  ensures BST_InOrder(tree) == result
+  // Ensures que Result esté ordenado
+  // Ensures que el tree tenga los mismos elementos que el result
+{
+  match tree {
+    case Leaf => List_Empty
+    case Node(left, x, right) => List_Concat(BST_InOrder(left), List_Concat(Cons(x, List_Empty), BST_InOrder(right)))
+  }
+}
+
+function method BST_ToSeq(tree:BST<T>) : seq<T>
+  decreases tree
+{
+  match tree {
+    case Leaf => []
+    case Node(left, x, right) => BST_ToSeq(left) + [x] + BST_ToSeq(right)
+  }
+}
+
+function method BST_ToSet(tree:BST<T>) : set<T>
+  decreases tree
+{
+  match tree {
+    case Leaf => {}
+    case Node(left, x, right) => BST_ToSet(left) + {x} + BST_ToSet(right)
+  }
+}
+
+function method BST_Contains(tree:BST<T>, d:T) : bool
+  decreases tree
+{
+  match tree {
+    case Leaf => false
+    case Node(left, x, rigth) => BST_Contains(left, d) || BST_Contains(rigth, d)
+  }
+}
+
+function method BST_Mirror(tree:BST<T>) : BST<T>
+  decreases tree
+{
+  match tree {
+    case Leaf => Leaf
+    case Node(left, x, right) => Node(BST_Mirror(right), x, BST_Mirror(left))
+  }
+}
+
+
+// ---------------------- Predicates ---------------------- //
+
+predicate bst_is_ordered(tree:BST<T>)
+  decreases tree
+{
+  match tree {
+    case Leaf => true
+    case Node(left, x, right) => 
+      bst_is_ordered(left) &&
+      bst_is_ordered(right) &&
+      (forall y :: y in BST_ToSet(left) ==> y < x) &&
+      (forall y :: y in BST_ToSet(right) ==> y >= x)
+  }
+}
+
+// ------------------------ Lemmas ------------------------ //
+
+/*
+lemma {:induction false} InOrderElemsSameThanTreeElemsLemma(tree:BST<T>, result:List<T>)
+  ensures List_ToSeq(BST_InOrder(tree)) == List_ToSeq(result)
+{
+  match tree {
+    case Leaf =>
+      calc == {
+        List_ToSeq(BST_InOrder(tree));
+          { assert BST_InOrder(tree) == List_Empty; }
+        List_ToSeq(List_Empty);
+          { assert List_Empty == result; }
+        List_ToSeq(result);
+      }
+    case Node(left, x, right) =>
+      calc == {
+        List_ToSeq(BST_InOrder(tree));
+          { assert List_ToSeq(BST_InOrder(tree)) == List_ToSeq(List_Concat(BST_InOrder(left), List_Concat(Cons(x, List_Empty), BST_InOrder(right)))); }
+        List_ToSeq(List_Concat(BST_InOrder(left), List_Concat(Cons(x, List_Empty), BST_InOrder(right))));
+          { assert List_ToSeq(List_Concat(BST_InOrder(left), List_Concat(Cons(x, List_Empty), BST_InOrder(right)))) == List_ToSeq(BST_InOrder(left)) + List_ToSeq(List_Concat(Cons(x, List_Empty), BST_InOrder(right))); }
+        List_ToSeq(BST_InOrder(left)) + List_ToSeq(List_Concat(Cons(x, List_Empty), BST_InOrder(right)));
+          { assert List_ToSeq(List_Concat(Cons(x, List_Empty), BST_InOrder(right))) == List_ToSeq(Cons(x, List_Empty)) + List_ToSeq(BST_InOrder(right)); }
+        List_ToSeq(BST_InOrder(left)) + List_ToSeq(Cons(x, List_Empty)) + List_ToSeq(BST_InOrder(right));
+          { assert List_ToSeq(BST_InOrder(left)) + List_ToSeq(Cons(x, List_Empty)) + List_ToSeq(BST_InOrder(right)) == List_ToSeq(BST_InOrder(left)) + [x] + List_ToSeq(BST_InOrder(right)); }
+        List_ToSeq(BST_InOrder(left)) + [x] + List_ToSeq(BST_InOrder(right));
+          { InOrderElemsSameThanTreeElemsLemma(left, result); }
+          { InOrderElemsSameThanTreeElemsLemma(right, result); }
+      }
+  }
+}
+*/
