test/data-types/binary-tree/BinaryTreeTest.dfy
@@ -1,44 +1,44 @@
-include "../../../src/data-types/binary-tree/BinaryTree.dfy"
+include "../../../src/data-types/binary-tree/BST.dfy"
 
 method Main() {
-  InOrderElemsTest();
+  InOrderTest();
   InsertTest();
   InsertWorstCaseTest();
   MirrorTest();
 }
 
-method InOrderElemsTest() {
-  var tree: BinaryTree<int> := Node(Node(Node(Leaf,1,Leaf),3,Leaf),4,Node(Node(Leaf, 5, Leaf),7,Leaf));
-  var list := BinaryTree_InOrderElems(tree);
+method InOrderTest() {
+  var tree: BST<int> := Node(Node(Node(Leaf,1,Leaf),3,Leaf),4,Node(Node(Leaf, 5, Leaf),7,Leaf));
+  var list := BST_InOrder(tree);
   var expected := Cons(1, Cons(3, Cons(4, Cons(5, Cons(7, List_Empty)))));
   assert(list == expected);
 }
 
 method InsertTest() {
-  var tree: BinaryTree<int> := Leaf;
-  tree := BinaryTree_Insert(tree, 4);
-  tree := BinaryTree_Insert(tree, 3);
-  tree := BinaryTree_Insert(tree, 1);
-  tree := BinaryTree_Insert(tree, 7);
-  tree := BinaryTree_Insert(tree, 5);
+  var tree: BST<int> := Leaf;
+  tree := BST_Insert(tree, 4);
+  tree := BST_Insert(tree, 3);
+  tree := BST_Insert(tree, 1);
+  tree := BST_Insert(tree, 7);
+  tree := BST_Insert(tree, 5);
   var expected := Node(Node(Node(Leaf,1,Leaf),3,Leaf),4,Node(Node(Leaf, 5, Leaf),7,Leaf));
   assert(tree == expected);
 }
 
 method InsertWorstCaseTest() {
-  var tree: BinaryTree<int> := Leaf;
-  tree := BinaryTree_Insert(tree, 1);
-  tree := BinaryTree_Insert(tree, 3);
-  tree := BinaryTree_Insert(tree, 4);
-  tree := BinaryTree_Insert(tree, 5);
-  tree := BinaryTree_Insert(tree, 7);
+  var tree := BST_Init();
+  tree := BST_Insert(tree, 1);
+  tree := BST_Insert(tree, 3);
+  tree := BST_Insert(tree, 4);
+  tree := BST_Insert(tree, 5);
+  tree := BST_Insert(tree, 7);
   var expected := Node(Leaf, 1, Node(Leaf, 3, Node(Leaf, 4, Node(Leaf, 5, Node(Leaf, 7, Leaf)))));
   assert(tree == expected);
 }
 
 method MirrorTest() {
-  var tree: BinaryTree<int> := Node(Node(Node(Leaf,1,Leaf),3,Leaf),4,Node(Node(Leaf, 5, Leaf),7,Leaf));
-  var mirroredTree := BinaryTree_Mirror(tree);
+  var tree: BST<int> := Node(Node(Node(Leaf,1,Leaf),3,Leaf),4,Node(Node(Leaf, 5, Leaf),7,Leaf));
+  var mirroredTree := BST_Mirror(tree);
   var expected := Node(Node(Leaf, 7, Node(Leaf, 5, Leaf)), 4, Node(Leaf, 3, Node(Leaf, 1, Leaf)));
   assert(mirroredTree == expected);
 }
